Forgot to send some files in last commit.  Now this should make completely.

certicoq/theories/L1_MalechaQuoted/wNorm.v
@@ -1,3 +1,8 @@
+(****)
+Add LoadPath "../common" as Common.
+Add LoadPath "../L1_MalechaQuoted" as L1.
+(****)
+
 Require Import Lists.List.
 Require Import Strings.String.
 Require Import Strings.Ascii.
@@ -20,12 +25,13 @@ Set Implicit Arguments.
 *** TRel is not itself a weak typed normal form, but unbound indices
 *** may occur under a binder in a weak typed normal form
 **)
+Section Sec_environ.
+Variable p:environ.
 Inductive WNorm: Term -> Prop :=
-| WNRel: forall n, WNorm (TRel n)
 | WNLam: forall nm ty bod, WNorm ty -> WNorm (TLambda nm ty bod)
 | WNProd: forall nm ty bod, WNorm ty -> WNorm (TProd nm ty bod)
-| WNFix: forall ds br, WNorm (TFix ds br)
-| WNAx: forall ty, WNorm (TAx ty)
+| WNFix: forall ds br, WDNorms ds -> WNorm (TFix ds br)
+| WNAx: forall nm, LookupAx nm p -> WNorm (TConst nm)
 | WNCase: forall mch n ty brs,
             WNorm mch -> WNorm ty -> WNorms brs -> ~ isCanonical mch ->
             WNorm (TCase n ty mch brs)
@@ -38,58 +44,77 @@ Inductive WNorm: Term -> Prop :=
            WNorm (TApp fn t ts)
 with WNorms: Terms -> Prop :=
 | WNtnil: WNorms tnil
-| WNtcons: forall t ts, WNorm t -> WNorms ts -> WNorms (tcons t ts).
-Hint Constructors WNorm WNorms.
+| WNtcons: forall t ts, WNorm t -> WNorms ts -> WNorms (tcons t ts)
+with WDNorms: Defs -> Prop :=
+| WDNtnil: WDNorms dnil
+| WDNtcons: forall t ds n s i,
+              WNorm t -> WNorm s -> WDNorms ds -> WDNorms (dcons n t s i ds).
+Hint Constructors WNorm WNorm WDNorms.
 Scheme WNorm_ind' := Induction for WNorm Sort Prop
-  with WNorms_ind' := Induction for WNorms Sort Prop.
-Combined Scheme WNormWNorms_ind from WNorm_ind', WNorms_ind'.
+      with WNorms_ind' := Induction for WNorms Sort Prop
+      with WDNorms_ind' := Induction for WDNorms Sort Prop.
+Combined Scheme WNormWNorms_ind
+         from WNorm_ind', WNorms_ind', WDNorms_ind' .
 
 Ltac rght := solve [right; intros h; inversion_Clear h; contradiction].
 Ltac lft := solve [left; constructor; assumption].
 
 (** WNorm is decidable **)
-Lemma WNorm_dec: 
+Lemma WNorm_dec:
   (forall t, WNorm t \/ ~ WNorm t) /\
   (forall ts, WNorms ts \/ ~ WNorms ts) /\
-  (forall (ds:Defs), True).
-apply TrmTrmsDefs_ind; intros; auto.
-- right. intros h. inversion h.
-- destruct H; [lft|rght].
-- destruct H; [lft|rght].
-- destruct H; rght.
-- destruct (isLambda_dec t). rght.
-  destruct (isFix_dec t). rght.
-  destruct (isApp_dec t). rght.
-  destruct H, H0, H1; try rght.
-  + left. apply WNApp; auto.
-- rght.
-- destruct H, H0, H1; try rght.
-  + destruct (isCanonical_dec t0); try rght.
-    * left. constructor; auto.
-- destruct H, H0; try rght.
-  + left; constructor; auto.
+  (forall (ds:Defs), WDNorms ds \/ ~ WDNorms ds).
+Proof.
+  apply TrmTrmsDefs_ind; intros; auto;
+  try (solve[right; intros h; inversion h]);
+  try (solve[left; constructor]).
+  - destruct H; [lft|rght].
+  - destruct H; [lft|rght].
+  - destruct (isLambda_dec t). rght.
+    destruct (isFix_dec t). rght.
+    destruct (isApp_dec t). rght.
+    destruct H, H0, H1; try rght.
+    + left. apply WNApp; auto.
+  - destruct (Lookup_dec s p).
+    + destruct H. destruct (isAx_dec x).
+      * left. constructor. subst. assumption.
+      * right. intros j. inversion j. elim H0.
+        unfold LookupAx in H2. apply (Lookup_functional H H2).
+    + right. intros h. inversion h. eelim H. apply H1.
+  - destruct H, H0, H1; try rght.
+    + destruct (isCanonical_dec t0); try rght.
+      * left. constructor; auto.
+  - destruct H; [lft|rght]. 
+  - destruct H, H0; try rght.
+    + left. constructor; assumption.
+  - destruct H, H0, H1; try rght.
+    + left. constructor; assumption.
 Qed.
 
 Lemma WNorms_tappendl:
   forall ts us, WNorms (tappend ts us) -> WNorms ts.
 Proof.
   induction ts; intros us h.
-  - constructor.
-  - simpl in h. apply WNtcons; inversion_Clear h.
+  - constructor.  - simpl in h. apply WNtcons; inversion_Clear h.
     + assumption.
     + eapply IHts. eassumption.
 Qed.
 
-
+(*******************
 Lemma Wcbv_WNorm:
-  forall p, WFaEnv p ->
+  WFaEnv p ->
     (forall t s, WcbvEval p t s -> WFapp t -> WNorm s) /\
     (forall ts ss, WcbvEvals p ts ss -> WFapps ts -> WNorms ss).
 Proof.
-intros p hp. apply WcbvEvalEvals_ind; simpl; intros; auto.
+intros hp. apply WcbvEvalEvals_ind; simpl; intros; auto.
 - inversion_Clear H0. intuition. 
 - inversion_Clear H0. intuition. 
 - inversion_Clear H0. apply H. assumption.
+- constructor.
+
+  assert (j:= Lookup_pres_WFapp hp l). inversion j. subst.   constructor.
+  unfold LookupAx in *.
+  simpl.
 - inversion_Clear H0. apply H.
   assert (j:= Lookup_pres_WFapp hp l). inversion j. assumption.
 - inversion_Clear H2. apply H1. 
@@ -111,6 +136,10 @@ intros p hp. apply WcbvEvalEvals_ind; simpl; intros; auto.
   + destruct H2 as [x0 [x1 [x2 j]]]. discriminate.
   + destruct H2 as [x0 [x1 j]]. discriminate.
   + destruct H2 as [x0 [x1 [x2 j]]]. discriminate.
+- inversion_Clear H2. constructor; intuition.
+  + destruct H2 as [x0 [x1 [x2 j]]]. discriminate.
+  + destruct H2 as [x0 [x1 j]]. discriminate.
+  + destruct H2 as [x0 [x1 [x2 j]]]. discriminate.
 - inversion_Clear H1. apply H0.
   refine (whCaseStep_pres_WFapp _ _ _ e); auto.
 - inversion_Clear H1. apply H0.
@@ -120,49 +149,44 @@ intros p hp. apply WcbvEvalEvals_ind; simpl; intros; auto.
   constructor; assumption.
 - inversion_Clear H1. constructor; intuition.
 Qed.
-
+**********************)
 
 Lemma wcbvEval_no_further:
-  forall p, 
     (forall t s, WcbvEval p t s -> WcbvEval p s s) /\
-    (forall ts ss, WcbvEvals p ts ss -> WcbvEvals p ss ss).
+    (forall ts ss, WcbvEvals p ts ss -> WcbvEvals p ss ss) /\
+    (forall ds es, WcbvDEvals p ds es -> WcbvDEvals p es es).
 Proof.
-  intros p. apply WcbvEvalEvals_ind; simpl; intros; auto.
+  apply WcbvEvalEvals_ind; simpl; intros; auto.
 Qed.
 
 
 (** If a program is in weak normal form, it has no wndEval step **)
 Lemma wNorm_no_wndStep_lem:
-  forall (p:environ),
   (forall t s, wndEval p t s -> ~ WNorm t) /\
-  (forall ts ss, wndEvals p ts ss -> ~ WNorms ts).
-intros p.
+  (forall ts ss, wndEvals p ts ss -> ~ WNorms ts) /\
+  (forall ds es, wndDEvals p ds es -> ~ WDNorms ds).
 apply wndEvalEvals_ind; intros; intros h;
 try (solve[inversion h]);
 try (solve[inversion h; subst; contradiction]).
+- inversion h. inversion l; subst;
+  unfold LookupDfn in l; unfold LookupAx in H0;
+    assert (j:=Lookup_functional l H0); discriminate.
 - inversion h. subst. elim H5. exists nm, ty, bod. reflexivity.
 - inversion h. subst. elim H6. constructor.
 - inversion h. subst. elim H6. constructor.
 - inversion h. subst. elim H6. exists dts, m. reflexivity.
-- destruct t; simpl in h; try (solve [elim H; constructor]).
-  + inversion w. subst.
-    * inversion h. subst. inversion H3.
-    * inversion h. subst. inversion H6.
-  + inversion h. subst. contradiction.
-  + inversion h. subst. contradiction.
-  + inversion h. subst. contradiction.
-  + elim H. inversion h. subst. assert (j:= WNorms_tappendl _ _ H5).
-    constructor; try assumption.
-  + inversion h. subst. contradiction.
-  + inversion h. subst. inversion H3. contradiction.
+- destruct t; simpl in h; inversion h; try (contradiction).
+  + subst. elim H. constructor; try assumption.
+    apply (WNorms_tappendl _ _ H5).
 Qed.
 
 Lemma wNorm_no_wndStep:
-  forall t, WNorm t -> forall p, no_wnd_step p t.
-unfold no_wnd_step, no_wnds_step, no_step. intros t h0 p b h1.
-elim (proj1 (wNorm_no_wndStep_lem p) _ _ h1). assumption.
+  forall t, WNorm t -> no_wnd_step p t.
+unfold no_wnd_step, no_wnds_step, no_step. intros t h0 b h1.
+elim (proj1 (wNorm_no_wndStep_lem) _ _ h1). assumption.
 Qed.
 
+End Sec_environ.
 
 (****
 Lemma no_wndStep_wNorm:
